Rewrite intro rules, cleanup, and more

LLVMState.thy
@@ -4,19 +4,126 @@ begin
 
 type_synonym state = "llvm_register_model * llvm_memory_model * llvm_memory_model"
 
-definition abs_memory :: "state \<Rightarrow> llvm_address \<Rightarrow> llvm_value option option" where
-  "abs_memory = undefined"
+
+section "Memory Abstraction for Proofs"
+
+definition abs_memory where
+  "abs_memory s a \<equiv> if valid_memory_address s a then 
+    case s!a of 
+      mem_val v \<Rightarrow> Some (Some v)
+    | mem_unset \<Rightarrow> Some None
+    | mem_freed \<Rightarrow> None
+  else None"
+
+fun memory_\<alpha> :: "state \<Rightarrow> llvm_address \<Rightarrow> llvm_value option option" where
+  "memory_\<alpha> (r,s,h) (saddr a) = abs_memory s a"
+| "memory_\<alpha> (r,s,h) (haddr a) = abs_memory h a"
+
+
+fun abs_memory_aux :: "state \<Rightarrow> llvm_address \<Rightarrow> llvm_value result" where
+  "abs_memory_aux (r,s,h) (saddr a) = get_memory s a"
+| "abs_memory_aux (r,s,h) (haddr a) = get_memory h a"
+
+definition memory_\<alpha>_old :: "state \<Rightarrow> llvm_address \<Rightarrow> llvm_value option option" where
+  "memory_\<alpha>_old s a = (case abs_memory_aux s a of
+    ok v \<Rightarrow> Some (Some v)
+  | err uninitialized_address \<Rightarrow> Some None
+  | _ \<Rightarrow> None)"
+
+lemma "memory_\<alpha>_old s a = memory_\<alpha> s a" 
+  unfolding memory_\<alpha>_old_def 
+  apply (cases a; cases s; auto split: option.splits result.splits simp: get_memory_def abs_memory_def)
+     apply (auto split: memory_value.splits)
+  done
 
 definition abs_value :: "state \<Rightarrow> llvm_value_ref \<Rightarrow> llvm_value option" where
   "abs_value = undefined"
 
+lemma wp_never_err_assert[wp_intro]:  "\<lbrakk> P; Q () \<rbrakk> \<Longrightarrow> wp (assert e P) Q"
+  apply (cases P) apply auto done
+
+lemma wp_get_memory[THEN consequence, wp_intro]: "abs_memory s a = Some (Some v) \<Longrightarrow> wp (get_memory s a) (\<lambda>r. r=v)"
+  unfolding get_memory_def
+  apply (intro wp_intro)
+   apply (split memory_value.split)
+   apply (auto simp: abs_memory_def split: if_splits)
+  done
+
+lemma wp_set_memory_update[THEN consequence, wp_intro]: "abs_memory s a \<noteq> None \<Longrightarrow> wp (set_memory s a v) (\<lambda>s'. abs_memory s' = (abs_memory s)(a := Some (Some v)))"
+  unfolding set_memory_def
+  apply (intro wp_intro)
+  by (auto split: if_splits simp: valid_memory_address_def abs_memory_def)
+
+
+
+(*
+do the same for get/set
+DO it for combined
+Also for allocate, was free before, now not etc.
+
+Have basic example for proof
+
+arrays :'D
+
+For related work:
+Look at existing memory models
+Hoare
+Separation logic
+Floyd's verification logic
+Peter's papers
+*)
+
+thm wp_intro
+
+
+lemma set_memory_abs:
+  assumes "set_memory h a v = ok h'"
+  shows "memory_\<alpha>_old (r, s, h') (haddr a) = Some (Some v)"
+  using assms
+  unfolding memory_\<alpha>_old_def set_memory_def apply simp
+  unfolding valid_memory_address_def get_memory_def by auto
+
+lemma abs_mem_ind:
+  assumes "set_memory h a v = ok h'"
+  shows "\<forall>a'. a' \<noteq> a \<longrightarrow> memory_\<alpha>_old (r,s,h) (haddr a') = memory_\<alpha>_old (r,s,h') (haddr a')"
+  using assms
+  unfolding memory_\<alpha>_old_def
+  by (simp add: memory_set_independent_get)
+
+lemma abs_mem_ind':
+  assumes "set_memory h a v = ok h'"
+  shows "\<forall>a'. a' \<noteq> a \<longrightarrow> ((memory_\<alpha>_old (r,s,h))((haddr a) := Some (Some v))) (haddr a') = memory_\<alpha>_old (r,s,h') (haddr a')"
+  using assms abs_mem_ind
+  by simp
+
+lemma abs_mem_ind'':
+  assumes "set_memory h a v = ok h'"
+  shows "\<forall>a'. ((memory_\<alpha>_old (r,s,h))((haddr a) := Some (Some v))) (saddr a') = memory_\<alpha>_old (r,s,h') (saddr a')"
+  using assms
+  by (simp add: memory_\<alpha>_old_def)
+
+lemma abs_memory_update_heap_forall:
+  assumes "set_memory h a v = ok h'"
+  shows "\<forall>a'. ((memory_\<alpha>_old (r, s, h))((haddr a) := Some (Some v))) a' = (memory_\<alpha>_old (r, s, h')) a'"
+  using assms set_memory_abs abs_mem_ind' abs_mem_ind''
+  apply auto
+  subgoal for a'
+    apply (cases a')
+    by auto
+  done
+
+lemma abs_memory_update_heap:
+  assumes "set_memory h a v = ok h'"
+  shows "((memory_\<alpha>_old (r, s, h))((haddr a) := Some (Some v))) = (memory_\<alpha>_old (r, s, h'))"
+  using assms abs_memory_update_heap_forall
+  by auto
 
 lemma store_value_abs:
   assumes "abs_value s vr = Some v"
   assumes "abs_value s pr = Some (addr a)"
   assumes "abs_memory s a \<noteq> None"
-  shows "wp_never_err (store_value s vr p) (\<lambda>s'. abs_value s' = abs_value s \<and> abs_memory s' = (abs_memory s)(a := Some (Some v)))"
-  sorry
+  shows "wp (store_value s vr p) (\<lambda>s'. abs_value s' = abs_value s \<and> abs_memory s' = (abs_memory s)(a := Some (Some v)))"
+  oops
 
 lemmas [wp_intro] = store_value_abs[THEN consequence]
 
