RegisterModel.thy
@@ -25,12 +25,7 @@ definition empty_register_model :: "('n, 'v) register_model" where
 
 section "Lemmas"
 
-lemma set_register_intro[wp_intro]:
-  assumes "\<exists>r'. set_register r name v = ok r'"
-  assumes "\<And>r'. set_register r name v = ok r' \<Longrightarrow> Q r'"
-  shows "wp_never_err (set_register r name v) Q"
-  using assms
-  by auto
+
 
 lemma register_empty_get_unknown: "get_register empty_register_model n = err unknown_register"
   unfolding get_register_def empty_register_model_def
@@ -46,35 +41,41 @@ lemma register_set_independent_get: "n \<noteq> n' \<Longrightarrow> set_registe
   unfolding get_register_def set_register_def
   by (cases "Mapping.lookup r n'"; auto)
 
-lemma register_set_independent_get_wp: "n \<noteq> n' \<Longrightarrow> wp_ignore_err (set_register r n' v) (\<lambda>r'. get_register r' n = get_register r n)"
+lemma register_set_independent_get_wlp: "n \<noteq> n' \<Longrightarrow> wlp (set_register r n' v) (\<lambda>r'. get_register r' n = get_register r n)"
   unfolding get_register_def set_register_def
-  by auto
+  apply (cases "Mapping.lookup r n'"; simp)
+  apply (intro wp_intro; simp)
+  by (intro wp_intro; simp)
 
 
 lemma register_set_get: "set_register r n v = ok r' \<Longrightarrow> get_register r' n = ok v"
   unfolding set_register_def get_register_def
   by (auto split: if_splits simp add: option.case_eq_if)
 
-lemma register_set_get_wp: "wp_ignore_err (do { r' \<leftarrow> set_register r n v; get_register r n }) ((=) v)"
+lemma register_set_get_wlp: "wlp (do { r' \<leftarrow> set_register r n v; get_register r n }) ((=) v)"
   unfolding set_register_def get_register_def
-  by (simp add: option.case_eq_if)
+  apply (cases "Mapping.lookup r n"; simp)
+  apply (intro wp_intro; simp)
+  by (intro wp_intro; simp)
 
 
 lemma register_get_override: "get_register r n = ok v \<Longrightarrow> set_register r n v' = err register_override"
   unfolding set_register_def get_register_def option.case_eq_if
   by (simp split: if_splits)
 
-lemma register_get_override_wp: "wp_ignore_err (get_register r n) (\<lambda>_. set_register r n v = err register_override)"
+lemma register_get_override_wlp: "wlp (get_register r n) (\<lambda>_. set_register r n v = err register_override)"
   unfolding get_register_def set_register_def
-  by auto
+  by (simp add: option.case_eq_if wp_intro)
 
 
 lemma register_set_override: "set_register r n v = ok r' \<Longrightarrow> set_register r' n v' = err register_override"
   unfolding set_register_def option.case_eq_if
   by (auto split: if_splits)
 
-lemma register_set_override_wp: "wp_ignore_err (set_register r n v) (\<lambda>r'. set_register r' n v' = err register_override)"
+lemma register_set_override_wlp: "wlp (set_register r n v) (\<lambda>r'. set_register r' n v' = err register_override)"
   unfolding get_register_def set_register_def
-  by auto
+  apply (cases "Mapping.lookup r n"; simp)
+  apply (intro wp_intro; simp)
+  by (intro wp_intro; simp)
 
 end
